\section{EOM Calculation}\label{app:eom}
Consider a quantum harmonic oscillator described by the Hamiltonian
\begin{equation}
    \hat{H} = \hbar \omega ( \ad \a + 1/2 ).
\end{equation}
Consider also that the quantum harmonic oscillator is subject to a temperature bath and is continuously measured. The system then evolves according to the master equation
\begin{equation}
    \dt \dmatrix = -\frac{i}{\hbar} [\hamiltonian, \dmatrix] + \gamma (\nbar + 1 ) \mathcal{D}[\a] \dmatrix + \gamma \nbar \mathcal{D}[\ad] \dmatrix + \lambda \mathcal{D}[\hat{A}] \dmatrix \label{eq:master}
\end{equation}
where $\gamma$ is the damping rate, $\nbar$ is the thermal occupancy defined as 
\begin{equation}
    \nbar = \frac{1}{e^{\hbar \omega / k_B T} - 1},
\end{equation}
$\lambda$ is the measurement rate, $\hat{A}$ is the measurement operator, and $\mathcal{D}[\hat{O}]$ is the Lindblad super operator defined as
\begin{equation}
    \mathcal{D}[\hat{O}] \dmatrix = \hat{O} \dmatrix \hat{O}^\dagger - \frac{1}{2} \{ \hat{O}^\dagger \hat{O}, \dmatrix \}.
\end{equation}
Then we also have the quadrature operators defined as 
\begin{equation}
    \hat{x} = \sqrt{\frac{\hbar}{2 m \omega}} (\a + \ad), \quad \hat{p} = i \sqrt{\frac{m \omega \hbar}{2}} (\a - \ad).
\end{equation}

We want to find the equations of motion when measuring the position quadrature
\begin{align}
    \dt\expval{\xop^2} &= \tr(\xop^2 \dt \dmatrix)\label{eq:x2} \\
    \dt\expval{\pop^2} &= \tr(\pop^2 \dt \dmatrix)\label{eq:p2}\\
    \dt\expval{\acomm{\xop}{\pop}} &= \tr(\acomm{\xop}{\pop} \dt \dmatrix). \label{eq:xp}
\end{align}
We start by defining the Liouvillian super operator
\begin{equation}
    \mathcal{L}\dmatrix = -\frac{i}{\hbar} [\hamiltonian, \dmatrix] + \gamma (\nbar + 1 ) \mathcal{D}[\a] \dmatrix + \gamma \nbar \mathcal{D}[\ad] \dmatrix
\end{equation}
which turns the master equation into
\begin{equation}
    \dt \dmatrix = \mathcal{L}\dmatrix + \lambda \mathcal{D}[\hat{x}] \dmatrix.
\end{equation}
\subsection{Solving for $\dt\expval{\xop^2}$}
We can write Eq. \eqref{eq:x2} as 
\begin{equation}
    \dt\expval{\xop^2} = \tr(\xop^2 \mathcal{L}\dmatrix) + \tr(\xop^2 \lambda \mathcal{D}[\hat{x}] \dmatrix)\label{eq:x2b}
\end{equation}
and then rewriting the left term using the creation and annihilation operators we get
\begin{align}
    \tr(\xop^2 \mathcal{L}\dmatrix) &= \frac{\hbar}{2m \omega} \tr((\a^2 + (\ad)^2 + \a\ad + \ad\a) \mathcal{L}\dmatrix )\\ 
    &= \frac{\hbar}{2 m \omega} \left[ \tr(\a^2 \mathcal{L}\dmatrix) + \tr((\ad)^2 \mathcal{L}\dmatrix) + \tr(\a\ad \mathcal{L}\dmatrix) + \tr(\ad\a \mathcal{L}\dmatrix)\right]
\end{align}
Solving these separately
\begin{align}
    \tr(\a^2 \mathcal{L} \dmatrix) &= -\frac{i}{\hbar}\tr(\a^2\comm{\hamiltonian}{\dmatrix}) + \gamma(\nbar + 1)\tr(\a^2 \mathcal{D}[\a]\dmatrix) + \gamma \nbar \tr(\a^2 \mathcal{D}[\ad]\dmatrix)\\
    &= -i\omega \tr(\a^2 \ad\a \dmatrix) + i \omega \tr(\a^2\dmatrix \ad\a)\\ 
    &+ \gamma(\nbar + 1) \tr(\a^3 \dmatrix \ad)- \frac{\gamma(\nbar + 1)}{2} \tr(\a^2\ad\a \dmatrix) - \frac{\gamma(\nbar + 1)}{2} \tr(\a^2 \dmatrix \ad\a)\\
    &+ \gamma \nbar \tr(\a^2\ad \dmatrix \a) - \frac{\gamma \nbar}{2} \tr(\a^3 \ad \dmatrix) - \frac{\gamma \nbar}{2} \tr(\a^2 \dmatrix \a\ad)
\end{align}
Using cyclic permutations of the trace and combining terms we get
\begin{align}
    \tr(\a^2 \mathcal{L} \dmatrix) &=  i\omega \tr(\comm{\ad\a}{\a^2}\dmatrix) + \frac{\gamma (\nbar + 1)}{2} \tr(\comm{\ad\a}{\a^2}\dmatrix) + \frac{\gamma \nbar}{2}\tr(\comm{\a^2}{\a\ad}\dmatrix)
\end{align}
The commutators are
\begin{align}
    \comm{\ad\a}{\a^2} &= \comm{\ad}{\a^2}\a = \a\comm{\ad}{\a}\a + \comm{\ad}{\a}\a^2 = -2 \a^2 \\
    \comm{\a^2}{\a\ad} &= \a\comm{\a^2}{\ad} = \a^2 \comm{\a}{\ad}+ \a\comm{\a}{\ad}\a = 2\a^2
\end{align}
Thus
\begin{align}
    \tr(\a^2 \mathcal{L} \dmatrix) &=  -2i\omega \tr(\a^2 \dmatrix) - \gamma(\nbar + 1) \tr(\a^2 \dmatrix) + \gamma \nbar \tr(\a^2 \dmatrix) = -(\gamma + 2i\omega) \tr(\a^2 \dmatrix)\\
    &= -(\gamma + 2i\omega) \expval{\a^2}.
\end{align}
By taking the hermition conjugate of the above we get
\begin{equation}
    \tr((\ad)^2 \mathcal{L} \dmatrix) = (\gamma - 2i\omega) \tr((\ad)^2 \dmatrix) = -(\gamma - 2i\omega) \expval{(\ad)^2}.
\end{equation}

Now we do the same for $\tr(\ad\a\mathcal{L}\dmatrix)$, so
\begin{align}
    \tr(\ad\a\mathcal{L}\dmatrix) &= -\frac{i}{\hbar}\tr(\ad\a\comm{\hamiltonian}{\dmatrix}) + \gamma(\nbar + 1)\tr(\ad\a\mathcal{D}[\a]\dmatrix) + \gamma \nbar \tr(\ad\a\mathcal{D}[\ad]\dmatrix)\\
    &= -i\omega \tr(\ad\a\ad\a\dmatrix) + i\omega \tr(\ad\a\dmatrix\ad\a)\\
    &+ \gamma(\nbar + 1)\tr(\ad\a^2\dmatrix\ad) - \frac{\gamma(\nbar + 1)}{2}\tr(\ad\a\ad\a\dmatrix) - \frac{\gamma(\nbar + 1)}{2}\tr(\ad\a\dmatrix\ad\a)\\
    &+ \gamma\nbar\tr(\ad\a\ad\dmatrix\a) - \frac{\gamma\nbar}{2}\tr(\ad\a^2\ad\dmatrix) - \frac{\gamma\nbar}{2}\tr(\ad\a\dmatrix\a\ad)
\end{align}
using cyclic permutations of the trace and combining terms we get
\begin{align}
    \tr(\ad\a\mathcal{L}\dmatrix) &= i\omega\tr(\comm{\ad\a}{\ad\a}\dmatrix) + \gamma(\nbar + 1) \tr((\ad)^2\a^2 \dmatrix) -\gamma (\nbar + 1)\tr(\ad\a\ad\a\dmatrix)\\
    &+ \gamma\nbar\tr(\a\ad\a\ad\dmatrix) - \frac{\gamma \nbar}{2} \tr(\ad\a^2\ad\dmatrix) - \frac{\gamma \nbar}{2} \tr(\a (\ad)^2 \a \dmatrix)
\end{align}
Commuting to simplify we get
\begin{align}
    \tr(\ad\a\mathcal{L}\dmatrix) &= - \gamma(\nbar + 1) \tr(\ad\a\dmatrix) - \gamma \nbar \tr(\comm{\a\ad}{\ad\a} \dmatrix) + \gamma \nbar \tr(\a\ad\dmatrix)
\end{align}
The commutator is equal to 0, and thus we get
\begin{equation}
    \tr(\ad\a\mathcal{L}\dmatrix) = - \gamma(\nbar + 1) \tr(\ad\a\dmatrix) +\gamma \nbar + \gamma\nbar \tr(\ad\a\dmatrix) = -\gamma \tr(\ad\a\dmatrix) + \gamma\nbar = -\gamma \expval{\ad\a} + \gamma\nbar.
\end{equation}
Similarly we can find that
\begin{equation}
    \tr(\a\ad\mathcal{L}\dmatrix) = -\gamma \tr(\a\ad\dmatrix) + \gamma(\nbar + 1) = -\gamma \expval{\a\ad} + \gamma(\nbar + 1).
\end{equation}
Then since $\xop^2$ commutes with $\xop$ (the measurement operator) we can write Eq. \eqref{eq:x2b} the equation of motion
\begin{align}
    \dt\expval{\xop^2} &= \tr(\xop^2\liouvillian\dmatrix) \\
    &= \frac{\hbar}{2 m \omega} \left( -(\gamma + 2 i \omega)\expval{\a^2} -(\gamma - 2 i \omega)\expval{(\ad)^2} - \gamma\expval{\ad\a} + \gamma\nbar - \gamma\expval{\a\ad} + \gamma(\nbar+1) \right)\\
    &= -\gamma \frac{\hbar}{2 m \omega} \left( \expval{\a^2} + \expval{(\ad)^2} + \expval{\ad\a} + \expval{\a\ad} \right) + \frac{i\hbar}{m}\left( \expval{(\ad)^2} - \expval{\a^2} \right) + \frac{\gamma \hbar}{m\omega}(\nbar + 1/2)
\end{align}
Since we have
\begin{equation}
    \acomm{\xop}{\pop} = i\hbar ((\ad)^2 - \a^2)
\end{equation}
We can write the equation of motion as
\begin{equation}
    \dt\expval{\xop^2} = - \gamma \expval{\xop^2} + \frac{1}{m}\expval{\acomm{\xop}{\pop}} + \frac{\gamma \hbar}{m\omega}(\nbar + 1/2)
\end{equation}

\subsection{Solving for $\dt\expval{\pop^2}$}
Writing Eq. \eqref{eq:p2} as 
\begin{equation}
    \dt\expval{\pop^2} = \tr(\pop^2 \mathcal{L}\dmatrix) + \tr(\pop^2 \lambda \mathcal{D}[\hat{x}] \dmatrix)\label{eq:p2b}
\end{equation}
Rewriting the left terms using $\a,\ad$ we get
\begin{align}
    \tr(\pop^2\liouvillian\dmatrix) &= -\frac{m\omega \hbar}{2} \tr((\a^2 + (\ad)^2 - \ad\a - \a\ad)\liouvillian\dmatrix)\\
    &= -\frac{m\omega \hbar}{2} \left( \tr(\a^2\liouvillian\dmatrix) + \tr((\ad)^2\liouvillian\dmatrix) - \tr(\ad\a\liouvillian\dmatrix) - \tr(\a\ad\liouvillian\dmatrix) \right)
\end{align}
We have solved for these before, so we can write 
\begin{align}
    \tr(\pop^2\liouvillian\dmatrix) &= -\frac{m\omega \hbar}{2} \left( -(\gamma + 2i\omega) \expval{\a^2} -(\gamma - 2i\omega) \expval{(\ad)^2} +\gamma \expval{\ad\a} - \gamma\nbar +\gamma \expval{\a\ad} - \gamma(\nbar + 1)  \right)\\
    &= -\gamma \expval{\pop^2} + m i\omega^2 \hbar \left( \expval{\a^2} - \expval{(\ad)^2} \right) + \gamma m \omega\hbar (\nbar + 1/2)\\
    &= -\gamma \expval{\pop^2} - m\omega^2 \expval{\acomm{\xop}{\pop}} + \gamma m \omega\hbar (\nbar + 1/2)
\end{align}

Solving the measurement term
\begin{align}
    \tr(\pop^2 \lambda \super{\xop} \dmatrix) &= \lambda \left( \tr(\pop^2 \xop \dmatrix \xop) - \frac{1}{2}\tr(\pop^2 \xop^2 \dmatrix) - \frac{1}{2} \tr(\pop^2 \dmatrix \xop^2) \right)\\
    &= \lambda \left( \tr(\xop \pop^2 \xop \dmatrix) - \frac{1}{2} \tr(\pop^2 \xop^2 \dmatrix) - \frac{1}{2} \tr(\xop^2 \pop^2 \dmatrix) \right)
\end{align}
Commuting the operators
\begin{align}
    \xop \pop^2 \xop &= \frac{1}{2}(\pop\xop + i\hbar)\pop\xop + \frac{1}{2}\xop\pop(\xop\pop -i\hbar) = \frac{1}{2}\pop\xop\pop\xop + \frac{1}{2} \xop\pop\xop\pop + \frac{i\hbar}{2} \comm{\pop}{\xop}\\
    &=\frac{1}{2}\pop\xop\pop\xop + \frac{1}{2} \xop\pop\xop\pop +\frac{\hbar^2}{2}\\
    \pop^2 \xop^2 &= \pop (\xop\pop -i\hbar)\xop = \pop\xop\pop\xop - i\hbar \pop\xop\\
    \xop^2 \pop^2 &= \xop(\pop\xop + i\hbar)\pop = \xop\pop\xop\pop + i\hbar \xop\pop
\end{align}
This gives 
\begin{align}
    \tr(\pop^2 \lambda \super{\xop} \dmatrix) &= \lambda \left(  \frac{1}{2}\tr(\pop\xop\pop\xop \dmatrix) + \frac{1}{2} \tr(\xop\pop\xop\pop\dmatrix) + \frac{\hbar^2}{2} -\frac{1}{2}\tr(\pop\xop\pop\xop \dmatrix) - \frac{1}{2} \tr(\xop\pop\xop\pop\dmatrix) + \frac{i\hbar}{2}\tr(\comm{\pop}{\xop}) \right)\\
    &= \frac{\lambda \hbar^2}{2} + \frac{\lambda i \hbar}{2} \tr(\comm{\pop}{\xop}) = \lambda \hbar^2
\end{align}

The final equation of motion then becomes
\begin{equation}
    \dt\expval{\pop^2} = -\gamma \expval{\pop^2} - m\omega^2 \expval{\acomm{\xop}{\pop}} + \gamma m \omega\hbar (\nbar + 1/2) + \lambda \hbar^2
\end{equation}

\subsection{Solving for $\dt\expval{\acomm{\xop}{\pop}}$}
Writing Eq. \eqref{eq:xp} as
\begin{equation}
    \dt\expval{\acomm{\xop}{\pop}} = \tr(\acomm{\xop}{\pop} \liouvillian \dmatrix) + \tr(\acomm{\xop}{\pop} \lambda \super{\xop} \dmatrix)
\end{equation}
Rewriting the left term as 
\begin{equation}
    \tr(\acomm{\xop}{\pop}\liouvillian \dmatrix) = i\hbar \tr((\a^2 - (\ad)^2)\liouvillian \dmatrix) = i\hbar \tr(\a^2 \liouvillian \dmatrix) - i\hbar \tr((\ad)^2 \liouvillian \dmatrix)
\end{equation}
We have calculated these terms before, so we can write
\begin{align}
    \tr(\acomm{\xop}{\pop}\liouvillian \dmatrix) &= -i\hbar \left(  (\gamma + 2i\omega) \expval{\a^2} - (\gamma - 2 i \omega) \expval{(\ad)^2} \right)\\
    &= -\gamma  i\hbar \left( \expval{\a^2} - \expval{(\ad)^2} \right) + 2\hbar\omega \left(\expval{\a^2} + \expval{(\ad)^2} \right)
\end{align}
We also have that
\begin{equation}
    \a^2 +(\ad)^2 = \frac{m\omega}{\hbar} \xop^2 - \frac{1}{m\omega \hbar} \pop^2
\end{equation}
Thus we get
\begin{equation}
    \tr(\acomm{\xop}{\pop}\liouvillian \dmatrix) =  -\gamma \expval{\acomm{\xop}{\pop}} + 2 m \omega^2 \expval{\xop^2} - \frac{2}{m} \expval{\pop^2}
\end{equation}
Solving for the measurement term
\begin{align}
    \lambda \tr(\acomm{\xop}{\pop}\super{\xop} \dmatrix) &= \frac{\lambda}{2} \left( \tr(\comm{\xop^2}{\pop\xop}\dmatrix) + \tr(\comm{\xop\pop}{\xop^2}) \right)
\end{align}
Solving the commutators shows that this will become zero.

\subsection{Results}
The final equations of motion are
\begin{align}
    \dt\expval{\xop^2} &= - \gamma \expval{\xop^2} + \frac{1}{m}\expval{\acomm{\xop}{\pop}} + \frac{\gamma \hbar}{m\omega}(\nbar + 1/2)\\
    \dt\expval{\pop^2} &= -\gamma \expval{\pop^2} - m\omega^2 \expval{\acomm{\xop}{\pop}} + \gamma m \omega\hbar (\nbar + 1/2) + \lambda \hbar^2\\
    \dt\expval{\acomm{\xop}{\pop}} &= -\gamma \expval{\acomm{\xop}{\pop}} + 2 m \omega^2 \expval{\xop^2} - \frac{2}{m} \expval{\pop^2}
\end{align}